\section{Mass and spring}
Ver imagen del muelle.

We try to obtain a function \(x(t)\), where \(x\) is the displacement of
the spring, that depends of \(F_a\), the force applied to the mass.

We might have friction, that we'll denote as \(F_f\), with the
corresponding friction coefficient that we'll denote as \(b\).

We know that:

\[ F_d = -k \cdot x \]
\[ F_f = b \cdot v \]
\[ \sum \vec{F} = m \cdot a \]

That gives:

\[ \sum \vec{F}(t) = F_a(t) - F_d(t) - F_f(t) = m \cdot a(t) \]

Substituting \(a(t)\) as \(\frac{\partial v(t)}{\partial t}\), and later
\(v\) as \(\frac{\partial x(t)}{\partial t}\):

\[ F_a(t) - k \cdot x(t) - b \cdot \frac{\partial x(t)}{\partial t} = m \cdot
\frac{\partial^2 x(t)}{\partial t^2} \]

Moving:

\[ F_a = m \cdot \frac{\partial^2 x(t)}{\partial t^2} + k \cdot x(t) - b \cdot
\frac{\partial x(t)}{\partial t} \]

Aplying the Laplace transform (assuming \(x(0) = 0\)):

\[ F_a(s) = m \cdot s^2 X(s) + k \cdot X(s) - b \cdot s \cdot X(s) \]

So we get:

\[ G(s) = \frac{X(s)}{F_a(s)} = \frac{1}{m \cdot s^2 + k - b \cdot s} \]
